Huge Language / Conversion refactors

src/Assembly/Pseudo.v
@@ -2,42 +2,43 @@ Require Import QhasmEvalCommon QhasmUtil State.
 Require Import Language.
 Require Import List.
 
-Module Type PseudoMachine.
-  Parameter width: nat.
-  Parameter vars: nat.
-  Parameter width_spec: Width width.
-End PseudoMachine.
+Module Pseudo <: Language.
+  Import EvalUtil ListState Util.
 
-Module Pseudo (M: PseudoMachine) <: Language.
-  Import EvalUtil ListState Util M.
-
-  Definition const: Type := word width.
-
-  (* Program Types *)
-  Inductive Pseudo: nat -> nat -> Type :=
-    (* Some true for registers, false for stack, None for default *)
+  Inductive Pseudo {w: nat} {spec: Width w}: nat -> nat -> Type :=
     | PVar: forall n, option bool -> Index n -> Pseudo n 1
     | PMem: forall n m, Index n -> Index m -> Pseudo n 1
-    | PConst: forall n, const -> Pseudo n 1
-
+    | PConst: forall n, word w -> Pseudo n 1
     | PBin: forall n, IntOp -> Pseudo n 2 -> Pseudo n 1
     | PDual: forall n, DualOp -> Pseudo n 2 -> Pseudo n 2
     | PCarry: forall n, CarryOp -> Pseudo n 2 -> Pseudo n 1
-    | PShift: forall n, RotOp -> Index width -> Pseudo n 1 -> Pseudo n 1
-
+    | PShift: forall n, RotOp -> Index w -> Pseudo n 1 -> Pseudo n 1
     | PIf: forall n m, TestOp -> Index n -> Index n -> Pseudo n m -> Pseudo n m -> Pseudo n m
     | PFunExp: forall n, Pseudo n n -> nat -> Pseudo n n
-
     | PLet: forall n k m, Pseudo n k -> Pseudo (n + k) m -> Pseudo n m
     | PComb: forall n a b, Pseudo n a -> Pseudo n b -> Pseudo n (a + b)
     | PCall: forall n m, Label -> Pseudo n m -> Pseudo n m.
 
   Hint Constructors Pseudo.
 
-  Definition Program := Pseudo vars vars.
-  Definition State := ListState width.
+  Record Params': Type := mkParams {
+    width: nat;
+    spec: Width width;
+    inputs: nat;
+    outputs: nat
+  }.
 
-  Fixpoint pseudoEval {n m} (prog: Pseudo n m) (st: State): option State :=
+  Definition Params := Params'.
+  Definition State (p: Params): Type := ListState (width p).
+  Definition Program (p: Params): Type :=
+    @Pseudo (width p) (spec p) (inputs p) (outputs p).
+
+  Definition Unary32: Params := mkParams 32 W32 1 1.
+  Definition Unary64: Params := mkParams 64 W64 1 1.
+
+  (* Evaluation *)
+
+  Fixpoint pseudoEval {n m w s} (prog: @Pseudo w s n m) (st: ListState w): option (ListState w) :=
     match prog with
     | PVar n _ i => omap (getVar i st) (fun x => Some (setList [x] st))
     | PMem n m v i => omap (getMem v i st) (fun x => Some (setList [x] st))
@@ -94,7 +95,7 @@ Module Pseudo (M: PseudoMachine) <: Language.
           else pseudoEval r st ))
 
     | PFunExp n p e =>
-      (fix funexpseudo (e': nat) (st': State) := 
+      (fix funexpseudo (e': nat) (st': ListState w) := 
         match e' with
         | O => Some st'
         | S e'' =>
@@ -105,94 +106,74 @@ Module Pseudo (M: PseudoMachine) <: Language.
     | PCall n m _ p => pseudoEval p st
     end.
 
-  Definition evaluatesTo := fun (p: Program) (st st': State) => (pseudoEval p st = Some st').
+  Definition evaluatesTo (p: Params) (prog: Program p) (st st': State p) :=
+      pseudoEval prog st = Some st'.
 
-  Module Notations.
-    Delimit Scope pseudo_notations with p.
-    Open Scope pseudo_notations.
+  Delimit Scope pseudo_notations with p.
+  Open Scope pseudo_notations.
 
-    Definition indexize (n: nat) (p: (n > 0)%nat) (x: nat): Index n.
-      intros; exists (x mod n);
-        abstract (pose proof (mod_bound_pos x n); omega).
-    Defined.
+  Definition indexize (n: nat) (p: (n > 0)%nat) (x: nat): Index n.
+    intros; exists (x mod n);
+      abstract (pose proof (mod_bound_pos x n); omega).
+  Defined.
 
-    Notation "% A" := (PVar _ (Some false) (indexize _ _ A))
-      (at level 20, right associativity) : pseudo_notations.
+  Notation "% A" := (PVar _ (Some false) (indexize _ _ A))
+    (at level 20, right associativity) : pseudo_notations.
 
-    Notation "$ A" := (PVar _ (Some true) (indexize _ _ A))
-      (at level 20, right associativity) : pseudo_notations.
+  Notation "$ A" := (PVar _ (Some true) (indexize _ _ A))
+    (at level 20, right associativity) : pseudo_notations.
 
-    Notation "'MEM' ( A , B )" :=  (PMem _ _ (indexize _ _ A) (indexize _ _ B))
-      (at level 20, right associativity) : pseudo_notations.
+  Notation "'MEM' ( A , B )" :=  (PMem _ _ (indexize _ _ A) (indexize _ _ B))
+    (at level 20, right associativity) : pseudo_notations.
 
-    Notation "# A" := (PConst _ (natToWord _ A))
-      (at level 20, right associativity) : pseudo_notations.
+  Notation "# A" := (PConst _ (natToWord _ A))
+    (at level 20, right associativity) : pseudo_notations.
 
-    Notation "A :+: B" := (PBin _ Add (PComb _ _ _ A B))
-      (at level 60, right associativity) : pseudo_notations.
+  Notation "A :+: B" := (PBin _ Add (PComb _ _ _ A B))
+    (at level 60, right associativity) : pseudo_notations.
 
-    Notation "A :+c: B" := (PCarry _ AddWithCarry (PComb _ _ _ A B))
-      (at level 60, right associativity) : pseudo_notations.
+  Notation "A :+c: B" := (PCarry _ AddWithCarry (PComb _ _ _ A B))
+    (at level 60, right associativity) : pseudo_notations.
 
-    Notation "A :-: B" := (PBin _ Sub (PComb _ _ _ A B))
-      (at level 60, right associativity) : pseudo_notations.
+  Notation "A :-: B" := (PBin _ Sub (PComb _ _ _ A B))
+    (at level 60, right associativity) : pseudo_notations.
 
-    Notation "A :&: B" := (PBin _ And (PComb _ _ _ A B))
-      (at level 45, right associativity) : pseudo_notations.
+  Notation "A :&: B" := (PBin _ And (PComb _ _ _ A B))
+    (at level 45, right associativity) : pseudo_notations.
 
-    Notation "A :^: B" := (PBin _ Xor (PComb _ _ _ A B))
-      (at level 45, right associativity) : pseudo_notations.
+  Notation "A :^: B" := (PBin _ Xor (PComb _ _ _ A B))
+    (at level 45, right associativity) : pseudo_notations.
 
-    Notation "A :|: B" := (PBin _ Or (PComb _ _ _ A B))
-      (at level 60, right associativity) : pseudo_notations.
+  Notation "A :|: B" := (PBin _ Or (PComb _ _ _ A B))
+    (at level 60, right associativity) : pseudo_notations.
 
-    Notation "A :>>: B" := (PShift _ Shr (indexize _ _ B) A)
-      (at level 60, right associativity) : pseudo_notations.
+  Notation "A :>>: B" := (PShift _ Shr (indexize _ _ B) A)
+    (at level 60, right associativity) : pseudo_notations.
 
-    Notation "A :<<: B" := (PShift _ Shl (indexize _ _ B) A)
-      (at level 60, right associativity) : pseudo_notations.
+  Notation "A :<<: B" := (PShift _ Shl (indexize _ _ B) A)
+    (at level 60, right associativity) : pseudo_notations.
 
-    Notation "A :**: B" := (PDual _ Mult (PComb _ _ _ A B))
-      (at level 55, right associativity) : pseudo_notations.
+  Notation "A :**: B" := (PDual _ Mult (PComb _ _ _ A B))
+    (at level 55, right associativity) : pseudo_notations.
 
-    Notation "'IF' O ( A , B ) 'THEN' L 'ELSE' R" :=
-      (PIf _ _ O (indexize _ _ A) (indexize _ _ B) L R)
-      (at level 70, left associativity) : pseudo_notations.
+  Notation "'IF' O ( A , B ) 'THEN' L 'ELSE' R" :=
+    (PIf _ _ O (indexize _ _ A) (indexize _ _ B) L R)
+    (at level 70, left associativity) : pseudo_notations.
 
-    Notation "'EXP' ( e ) ( F )" :=
-      (PFunExp _ F e)
-      (at level 70, left associativity) : pseudo_notations.
+  Notation "'EXP' ( e ) ( F )" :=
+    (PFunExp _ F e)
+    (at level 70, left associativity) : pseudo_notations.
 
-    Notation "'LET' E 'IN' F" :=
-      (PLet _ _ _ E F)
-      (at level 70, left associativity) : pseudo_notations.
+  Notation "'LET' E 'IN' F" :=
+    (PLet _ _ _ E F)
+    (at level 70, left associativity) : pseudo_notations.
 
-    Notation "A | B" :=
-      (PComb _ _ _ A B)
-      (at level 65, left associativity) : pseudo_notations.
+  Notation "A | B" :=
+    (PComb _ _ _ A B)
+    (at level 65, left associativity) : pseudo_notations.
 
-    Notation "'CALL' n ::: A" :=
-      (PCall _ _ n A)
-      (at level 65, left associativity) : pseudo_notations.
-
-    Definition p0: Pseudo 1 2.
-      refine (CALL 0 ::: %0 :**: $0); intuition.
-    Defined.
-  End Notations.
-
-  (* world peace *)
+  Notation "'CALL' n ::: A" :=
+    (PCall _ _ n A)
+    (at level 65, left associativity) : pseudo_notations.
 End Pseudo.
 
-Module PseudoUnary32 <: PseudoMachine.
-  Definition width := 32.
-  Definition vars := 1.
-  Definition width_spec := W32.
-  Definition const: Type := word width.
-End PseudoUnary32.
-
-Module PseudoUnary64 <: PseudoMachine.
-  Definition width := 64.
-  Definition vars := 1.
-  Definition width_spec := W64.
-  Definition const: Type := word width.
-End PseudoUnary64.
