src/Assembly/PseudoConversion.v
@@ -1,0 +1,220 @@
+
+Require Export Language Conversion QhasmEvalCommon QhasmUtil.
+Require Export Pseudo AlmostQhasm State.
+Require Export Bedrock.Word NArith NPeano Euclid.
+Require Export List Sumbool Vector.
+
+Module PseudoConversion <: Conversion Pseudo AlmostQhasm.
+  Import QhasmCommon AlmostQhasm EvalUtil Util Pseudo StateCommon.
+  Import ListNotations.
+
+  Definition MMap {w} := NatM.t (Mapping w).
+  Definition mempty {w} := NatM.empty (Mapping w).
+
+  Definition FMap {w} := NatM.t (AlmostProgram * (list (Mapping w))).
+  Definition fempty {w} := NatM.empty (AlmostProgram * (list (Mapping w))).
+
+  Definition getStart {w s n m} (prog: @Pseudo w s n m) :=
+    let ns := (fix getStart' {n' m'} (p': @Pseudo w s n' m') :=
+      match p' with
+      | PVar _ _ i => [proj1_sig i]
+      | PBin _ _ p => getStart' p
+      | PDual _ _ p => getStart' p
+      | PCarry _ _ p => getStart' p
+      | PShift _ _ _ p => getStart' p
+      | PIf _ _ _ _ _ l r => (getStart' l) ++ (getStart' r)
+      | PFunExp _ p _ => getStart' p
+      | PLet _ k _ a b => (n + k) :: (getStart' a) ++ (getStart' b)
+      | PComb _ _ _ a b => (getStart' a) ++ (getStart' b)
+      | PCall _ _ _ p => getStart' p
+      | _ => []
+      end) _ _ prog in
+
+    maxN (n :: m :: ns).
+
+  Definition addMap {T} (a b: NatM.t T): NatM.t T :=
+    (fix add' (m: NatM.t T) (elts: list (nat * T)%type) :=
+      match elts with
+      | [] => m
+      | (k, v) :: elts' => add' (NatM.add k v m) elts'
+      end) a (NatM.elements b).
+
+  Fixpoint convertProgram' {n m} (prog: Pseudo n m) (start: nat) (M: MMap) (F: FMap):
+      option (AlmostProgram * (list (Mapping width)) * MMap * FMap) :=
+    let rM := fun (x: nat) => regM _ (reg width_spec x) in
+    let sM := fun (x: nat) => stackM _ (stack width_spec x) in
+
+    let reg' := reg width_spec in
+    let stack' := stack width_spec in
+    let const' := const width_spec in
+
+    let G := fun (k: nat) =>
+      match (NatM.find k M) with
+      | Some v => v
+      | _ => rM k (* TODO: more intelligent defaults *)
+      end in
+
+    let madd := fun (k: nat) (f: nat -> Mapping width) => NatM.add k (f k) in
+    let fadd := fun (k: nat) (f: AlmostProgram) (r: list (Mapping width)) => NatM.add k (f, r) in
+
+    match prog with
+    | PVar n (Some true) i => Some (ASkip, [rM i], madd i rM M, F)
+    | PVar n (Some false) i => Some (ASkip, [sM i], madd i sM M, F)
+    | PVar n None i => Some (ASkip, [G i], M, F) 
+
+    | PConst n c => Some (AAssign (AConstInt (reg' start) (const' c)),
+                         [rM start], madd start rM M, F)
+
+    | PMem n m v i => Some (AAssign (ARegMem (reg' start) (mem width_spec v) i),
+                           [rM start], madd start rM M, F)
+
+    | PBin n o p =>
+      match (convertProgram' p start M F) with
+      | Some (p', [regM (reg _ _ a); regM (reg _ _ b)], M', F') =>
+        Some (ASeq p' (AOp (IOpReg o (reg' a) (reg' b))),
+              [rM a], madd a rM (madd b rM M'), F')
+
+      | Some (p', [regM (reg _ _ a); constM c], M', F') =>
+        Some (ASeq p' (AOp (IOpConst o (reg' a) c)),
+              [rM a], madd a rM M', F')
+
+      | Some (p', [regM (reg _ _ a); memM _ b i], M', F') =>
+        Some (ASeq p' (AOp (IOpMem o (reg' a) b i)),
+              [rM a], madd a rM M', F')
+
+      | Some (p', [regM (reg _ _ a); stackM (stack _ _ b)], M', F') =>
+        Some (ASeq p' (AOp (IOpStack o (reg' a) (stack' b))),
+              [rM a], madd a rM (madd b sM M'), F')
+
+      | _ => None
+      end
+
+    | PCarry n o p =>
+      match (convertProgram' p start M F) with
+      | Some (p', [regM (reg _ _ a); regM (reg _ _ b)], M', F') =>
+        Some (ASeq p' (AOp (COp o (reg' a) (reg' b))),
+              [rM a], madd a rM (madd b rM M'), F')
+
+      | _ => None
+      end
+
+    | PDual n o p =>
+      match (convertProgram' p (S start) M F) with
+      | Some (p', [regM (reg _ _ a); regM (reg _ _ b)], M', F') =>
+        Some (ASeq p' (AOp (DOp o (reg' a) (reg' b) (Some (reg' start)))),
+              [rM a; rM start], madd a rM (madd b rM (madd start rM M')), F')
+
+      | _ => None
+      end
+
+    | PShift n o x p =>
+      match (convertProgram' p start M F) with
+      | Some (p', [regM (reg _ _ a)], M', F') =>
+        Some (ASeq p' (AOp (ROp o (reg' a) x)),
+              [rM a], madd a rM M', F')
+
+      | _ => None
+      end
+
+    | PLet n k m f g =>
+      match (convertProgram' f start M F) with
+      | None => None
+      | Some (fp, fm, M', F') =>
+        match (convertProgram' g (start + (length fm)) M' F') with
+        | None => None
+        | Some (gp, gm, M'', F'') => Some (ASeq fp gp, gm, M'', F'')
+        end
+      end
+
+    | PComb n a b f g => 
+      match (convertProgram' f start M F) with
+      | None => None
+      | Some (fp, fm, M', F') =>
+        match (convertProgram' g (start + (length fm)) M' F') with
+        | None => None
+        | Some (gp, gm, M'', F'') => Some (ASeq fp gp, fm ++ gm, M'', F'')
+        end
+      end
+
+    | PIf n m o i0 i1 l r => 
+      match (convertProgram' l start M F) with
+      | None => None
+      | Some (lp, lr, lM, lF) =>
+
+        match (convertProgram' r start lM lF) with
+        | None => None
+        | Some (rp, rr, M', F') =>
+
+          if (list_eq_dec mapping_dec lr rr)
+          then
+            match (G (proj1_sig i0), G (proj1_sig i1)) with
+            | (regM r0, regM r1) => Some (ACond (CReg _ o r0 r1) lp rp, lr, M', F')
+            | (regM r, constM c) => Some (ACond (CConst _ o r c) lp rp, lr, M', F')
+            | _ => None
+            end
+          else None
+        end
+      end
+
+    | PFunExp n f e => 
+      match (convertProgram' f (S start) M F) with
+      | Some (fp, fr, M', F') => 
+        let a := start in
+        Some (ASeq
+          (AAssign (AConstInt (reg' a) (const' (natToWord _ O))))
+          (AWhile (CConst _ TLt (reg' a) (const' (natToWord _ e)))
+            (ASeq fp (AOp (IOpConst Add (reg' a) (const' (natToWord _ 1)))))),
+          fr, madd a rM M', F')
+
+      | _ => None
+      end
+ 
+    | PCall n m lbl f =>
+      match (convertProgram' f start M F) with
+      | Some (fp, fr, M', F') =>
+        let F'' := NatM.add lbl (fp, fr) F' in
+        Some (ACall lbl, fr, M', F'')
+      | None => None
+      end
+    end.
+
+  Definition convertProgram (prog: Pseudo inVars outVars): option AlmostProgram := 
+    match (convertProgram' prog (max inVars outVars) mempty fempty) with
+    | Some (prog', _, M, F) =>
+      Some (fold_left
+           (fun p0 t => match t with | (k, (v, _)) => ADef k v p0 end)
+           prog'
+           (of_list (NatM.elements F)))
+    | _ => None
+    end.
+
+  Fixpoint convertState (st: AlmostQhasm.State): option State :=
+    let vars := max inVars outVars in
+
+    let try_cons := fun {T} (x: option T) (l: list T) =>
+      match x with | Some x' => x' :: l | _ => l end in
+
+    let get := fun i =>
+      match (FullState.getReg (reg width_spec i) st,
+             FullState.getStack (stack width_spec i) st) with
+      | (Some v, _) => Some v
+      | (_, Some v) => Some v
+      | _ => None
+      end in
+
+    let varList := (fix cs' (n: nat) :=
+      try_cons (get (vars - n)) (match n with | O => [] | S m => cs' m end)) vars in
+
+    match st with
+    | FullState.fullState _ _ memState _ carry =>
+      if (Nat.eq_dec (length varList) vars)
+      then Some (varList, memState, carry)
+      else None
+    end.
+
+  Lemma convert_spec:  forall a a' b b' prog prog',
+    convertProgram prog = Some prog' ->
+    convertState a = Some a' -> convertState b = Some b' ->
+    AlmostQhasm.evaluatesTo prog' a b <-> evaluatesTo prog a' b'.
+  Admitted.
+End PseudoConversion.
